Almost got unicity of sorting, needs work on sigmas and projections

proof/CCPD.alaChen/Generation.v
@@ -37,313 +37,274 @@ unfold is_prop in H1.
 induction H1 ; discriminate.
 Qed.
 
-Fixpoint prod_sort (t : term) : term :=
+Lemma typ_not_kind2 : forall G T, ~ G |- Srt kind : T.
+Proof.
+  unfold not ; intros.
+  apply (typ_not_kind H).
+  auto.
+Qed.
+
+Hint Resolve lift_eq_sort typ_not_kind2 : coc.
+
+
+Fixpoint type_range (t : term) : term :=
   match t with
-  | Prod U V => prod_sort V
+  | Prod U V => type_range V
+  | Sum U V => type_range V
   | _ => t
   end.
 
-Inductive prod_target : term -> nat -> term -> Prop :=
-| prod_target_S : forall U V T n, prod_target V n T -> prod_target (Prod U V) (S n) (lift 1 T)
-| prod_target_0 : forall T, forall U V, T <> Prod U V -> prod_target T 0 T.
+Definition type_dom (t : term) : term :=
+  match t with
+  | Prod U V => type_range U
+  | Sum U V => type_range U
+  | _ => type_range t
+  end.
 
-Definition prod_dec : forall t, {exists U, exists V, t = Prod U V} + {forall U V, t <> Prod U V}.
-Proof.
-intros.
-induction t ; try solve [right ; intros ; red ; intros ; discriminate].
-left.
-exists t1 ; exists t2 ; reflexivity.
-Qed.
+Fixpoint type_no_kind (t : term) : Prop :=
+  match t with
+  | Prod U V => type_no_kind U /\ type_no_kind V
+  | Sum U V => type_no_kind U /\ type_no_kind V
+  | Srt kind => False
+  | _ => True
+  end.
 
-Lemma inv_lift_sort : forall t s n, lift n t = Srt s -> t = Srt s.
-Proof.
-intros.
-induction t ; simpl ; try discriminate.
-unfold lift in H ; simpl in H.
-auto.
-Qed.
-
-Lemma inv_lift_prod : forall t U V n, lift n t = Prod U V ->
- exists U', exists V', t = Prod U' V' /\ U = (lift_rec n U' 0) /\ V = (lift_rec n V' 1).
-Proof.
-intros.
-induction t ; simpl ; try discriminate.
-unfold lift in H ; simpl in H.
-injection H ; intros.
-exists t1 ; exists t2 ; split ; [auto | split ; auto].
-Qed.
-
-Lemma inv_lift_sum : forall t U V n, lift n t = Sum U V ->
- exists U', exists V', t = Sum U' V' /\ U = (lift_rec n U' 0) /\ V = (lift_rec n V' 1).
-Proof.
-intros.
-induction t ; simpl ; try discriminate.
-unfold lift in H ; simpl in H.
-injection H ; intros.
-exists t1 ; exists t2 ; split ; [auto | split ; auto].
-Qed.
-
-Lemma inv_lift_subset : forall t U V n, lift n t = Subset U V ->
- exists U', exists V', t = Subset U' V' /\ U = (lift_rec n U' 0) /\ V = (lift_rec n V' 1).
-Proof.
-intros.
-induction t ; simpl ; try discriminate.
-unfold lift in H ; simpl in H.
-injection H ; intros.
-exists t1 ; exists t2 ; split ; [auto | split ; auto].
-Qed.
-
-Lemma inv_lift_abs : forall t U V n, lift n t = Abs U V ->
- exists U', exists V', t = Abs U' V' /\ U = (lift_rec n U' 0) /\ V = (lift_rec n V' 1).
-Proof.
-intros.
-induction t ; simpl ; try discriminate.
-unfold lift in H ; simpl in H.
-injection H ; intros.
-exists t1 ; exists t2 ; split ; [auto | split ; auto].
-Qed.
-
-Lemma inv_lift_app : forall t U V n, lift n t = App U V ->
- exists U', exists V', t = App U' V' /\ U = (lift_rec n U' 0) /\ V = (lift_rec n V' 0).
-Proof.
-intros.
-induction t ; simpl ; try discriminate.
-unfold lift in H ; simpl in H.
-injection H ; intros.
-exists t1 ; exists t2 ; split ; [auto | split ; auto].
-Qed.
-(*
-Lemma prod_no_kind : forall t G T, G |- t : T -> 
-  forall U V, t = Prod U V -> ~ (exists n, prod_target t n (Srt kind)).*)
-
-(*Ltac doubleind t := induction t as [dH1] ; induction dH1 as [dH2].*)
-
-Lemma prod_target_not_kind : forall t G T, G |- t : T -> 
-  forall U V, t = Prod U V -> ~ (exists n, prod_target t n (Srt kind)).
-Proof.
-induction t ; try solve [unfold prod_sort ; red ; intros ; try discriminate].
-intros.
-induction (prod_dec V).
-induction a.
-induction H1.
-red ; intros.
-rewrite H0 in H2.
-simpl in H2.
-injection H0.
-intros.
-rewrite H3 in IHt2.
-
-induction H ; try discriminate.
-
-injection H0 ; intros.
-rewrite H7 in H5.
-rewrite H6 in H5.
-apply (IHt2 _ _ H5 _ _ H1).
-induction H2.
-inversion H2.
-pose (inv_lift_sort T0 1 H12).
-rewrite e0 in H11.
-exists n ; rewrite H12 ; apply H11.
-
-apply (IHtyp1 H0).
-
-injection H0 ; intros.
-rewrite H1 in IHt2.
-induction H ; try discriminate.
-injection H0 ; intros.
-rewrite H4 in H3.
-
-red ; intros.
-
-simpl in H6.
-rewrite H4 in H6.
-induction H6.
-inversion H6.
-pose (inv_lift_sort T0 1 H11).
-induction V ; try solve [
-  inversion H10 ; rewrite H15 in H3 ; rewrite e0 in H3 ; apply (typ_not_kind H3) ; auto ].
-clear IHV1 ; clear IHV2.
-
-apply (b V1 V2) ; auto.
-
-apply IHtyp1 ; auto.
-Qed.
-(* 
-Lemma typ_sort : forall G t T, G |- t : T -> T <> Srt kind -> 
-  exists s, G |- T : Srt s.
-Proof.
-  induction 1 ; simpl ; intros ; auto with coc.
-
-  elim H0 ; auto.
-
-  elim H0 ; auto.
-  
-  exact (wf_sort_lift n e T H H0).
-  
-  destruct (IHtyp3 (typ_not_kind H0)).
-  exists x.
-  apply type_prod with s1 ; auto with coc core.
-
-  assert(Prod V Ur <> Srt kind) ; unfold not ; intros ; try discriminate.
-  destruct (IHtyp2 H2).
-  exists x.
-*)
-
-Lemma prod_arity_not_kind : forall G t T, G |- t : T -> 
-  prod_sort t <> Srt kind.
+Lemma type_has_no_kind : forall G t T, G |- t : T -> type_no_kind t.
 Proof.
   induction 1; simpl ; intros ; auto with coc ; try discriminate.
 Qed.
 
-Lemma prod_lift_to_sort : forall n t k s, prod_sort (lift_rec n t k) = Srt s -> prod_sort t = Srt s.
+Lemma type_no_kind_not_kind : forall t, type_no_kind t -> t <> Srt kind.
 Proof.
-  induction t ; simpl ; intros ; try discriminate.
-  assumption.
-  generalize H ; elim (le_gt_dec k n0) ; intros ; simpl in H0 ; discriminate.
+  induction t ; unfold not ; intros ; try discriminate.
+  simpl in H.
+  inversion H0.
+  rewrite H2 in H.
+  auto.
+Qed.
+(*
+Lemma type_range_not_kind_ps : forall G t T, G |- t : T -> 
+  forall U V, t = Prod U V \/ t = Sum U V -> type_range U <> Srt kind /\
+  type_range V <> Srt kind.
+Proof.
+  induction 1; simpl ; intros ; auto with coc ; try (intuition ; discriminate).
+  destruct H1.
+
+  inversion H1.
+  rewrite <- H3.
+  rewrite <- H4.
+  split.
+  apply (type_range_not_kind H).
+  apply (type_range_not_kind H0).
+  discriminate.
+
+  inversion H1.
+  discriminate.
+  inversion H2.
+  rewrite <- H4.
+  rewrite <- H5.
+  split.
+  apply (type_range_not_kind H).
+  apply (type_range_not_kind H0).
+Qed.
+*)
+Lemma lift_type_range_eq_sort : forall n t k, type_no_kind (lift_rec n t k) -> 
+  type_no_kind t.
+Proof.
+  induction t ; simpl ; intros ; try discriminate ; auto.
+
+  intuition.
+  apply IHt1 with k ; auto.
+  apply IHt2 with (S k) ; auto.
+
+  intuition.
+  apply IHt1 with k ; auto.
   apply IHt2 with (S k) ; auto.
 Qed.
 
-Lemma prod_subst_to_sort : forall u v n, prod_sort u <> Srt kind ->
-  prod_sort v <> Srt kind -> prod_sort (subst_rec u v n) <> Srt kind.
+Lemma type_no_kind_lift : forall n t k, type_no_kind t ->
+  type_no_kind (lift_rec n t k).
 Proof.
-  induction v ; simpl ; intros ; try discriminate.
-  assumption.
+  induction t ; simpl ; intros ; try discriminate ; auto.
+
+  elim (le_gt_dec k n0) ; simpl ; intros ; auto.
+  intuition.
+  intuition.
+Qed.
+
+Lemma type_range_subst_not_kind : forall u v n, type_no_kind u ->
+  type_no_kind v -> type_no_kind (subst_rec u v n).
+Proof.
+  induction v ; simpl ; intros ; try discriminate ; auto.
+
   elim (lt_eq_lt_dec n0 n) ; intros.
-  induction a ; simpl ; intros ; unfold not ; intros ; try discriminate.
-  unfold lift in H1.
-  pose (prod_lift_to_sort n0 u 0 H1).
-  contradiction.
-  simpl ; unfold not ; intros ; discriminate.
-  
-  apply IHv2 ; auto with coc.
+  induction a ; simpl ; intros ; unfold not ; intros ; try discriminate ; auto.
+  unfold lift ; apply (type_no_kind_lift); auto.
+  auto.
+
+  intuition.
+  intuition.
 Qed.
  
-Lemma prod_arity_not_kind_type : forall G t T, G |- t : T -> 
-  forall U V, T = Prod U V -> prod_sort V <> Srt kind.
+Lemma type_no_kind_type : forall G t T, G |- t : T -> 
+  forall U V, (T = Prod U V \/ T = Sum U V) -> type_no_kind T.
 Proof.
   induction 1 using typ_mutwf with
   (P := fun G t T => fun H : G |- t : T =>
-    forall U V, T = Prod U V -> prod_sort V <> Srt kind)
+  forall U V, (T = Prod U V \/ T = Sum U V) -> type_no_kind T)
   (P0 := fun G U V s => fun H : G |- U >> V : s => True (*
     (forall X Y, U = Prod X Y -> prod_sort Y <> Srt kind) /\
     (forall X Y, U = Prod X Y -> prod_sort Y <> Srt kind)*))
   (P1 := fun e => fun H : wf e => 
-    forall U V n, item_lift (Prod U V) e n -> prod_sort V <> Srt kind) 
- ; simpl ; intros ; auto with coc ; try discriminate.
+    forall T n, item_lift T e n -> 
+    forall U V, (T = Prod U V \/ T = Sum U V) -> type_no_kind T)
+ ; simpl ; intros ; auto with coc ; try discriminate ; 
+ try (destruct H ; discriminate) ;  try (destruct H1 ; discriminate).
 
-  apply IHtyp with U n. 
-  rewrite H in i ; assumption.
+  apply IHtyp with n U V ; auto.
 
+  destruct H2 ; try discriminate.
   assert (e |- Prod T U : Srt s2).
   apply type_prod with s1 ; auto with coc.
-  rewrite H2 in H3.
-  pose (prod_arity_not_kind H3) ; auto with coc.
+  pose (type_has_no_kind H3) ; auto with coc.
+
+  destruct H1.
+  induction Ur ;  try (unfold subst, subst_rec ; simpl ; intros ; discriminate).
+  unfold subst in H1.
+  generalize H1 ; clear H1.
+  unfold subst_rec ; elim (lt_eq_lt_dec 0 n).
+  intro a ; case a ; clear a ; intros ; try discriminate.
+  rewrite <- e0 ; simpl.
+  unfold subst ; simpl.
+  rewrite lift0.
+  apply (type_has_no_kind H) ; auto with coc.
+
+  intros ; discriminate.
+  pose (IHtyp2 V (Prod Ur1 Ur2) (or_introl _ (refl_equal (Prod V (Prod Ur1 Ur2))))).
+  simpl in t.
+  destruct t.
+  destruct H3.
+  unfold subst in H1 ; simpl in H1.
+  clear IHUr1 IHUr2.
+
+  inversion H1.
+
+  pose (type_has_no_kind H).
+  split ; apply type_range_subst_not_kind ; auto.
 
   induction Ur ;  try (unfold subst, subst_rec ; simpl ; intros ; discriminate).
   unfold subst in H1.
   generalize H1 ; clear H1.
   unfold subst_rec ; elim (lt_eq_lt_dec 0 n).
   intro a ; case a ; clear a ; intros ; try discriminate.
-  rewrite lift0 in H1.
-  rewrite H1 in H.
-  pose (prod_arity_not_kind H) ; auto with coc.
+  rewrite <- e0 ; simpl.
+  unfold subst ; simpl.
+  rewrite lift0.
+  apply (type_has_no_kind H) ; auto with coc.
 
   intros ; discriminate.
-  pose (IHtyp2 V (Prod Ur1 Ur2) (refl_equal (Prod V (Prod Ur1 Ur2)))).
-  simpl in n.
+  pose (IHtyp2 V (Sum Ur1 Ur2) (or_introl _ (refl_equal (Prod V (Sum Ur1 Ur2))))).
+  simpl in t.
+  destruct t.
+  destruct H3.
   unfold subst in H1 ; simpl in H1.
   clear IHUr1 IHUr2.
 
   inversion H1.
 
-  pose (prod_arity_not_kind H).
-  apply prod_subst_to_sort ; auto.
+  pose (type_has_no_kind H).
+  split ; apply type_range_subst_not_kind ; auto.
 
+  destruct H3.
+  discriminate.
+  inversion H3.
+  rewrite <- H6.
+  rewrite <- H5.
+  split ; [apply (type_has_no_kind H) | apply (type_has_no_kind H1)].
   
+  pose (IHtyp U V (or_intror _ (refl_equal (Sum U V)))).
+  simpl in t0.
+  intuition.
   
-  Focus 3.
-  induction M ; simpl in H3 ; try discriminate.
-  generalize H3 ; unfold subst, subst_rec.
+  assert(type_no_kind (Pi1 t)) ; auto with coc.
+  simpl ; auto.
+  unfold subst ; apply type_range_subst_not_kind ; auto.
+  intuition.
+  pose (IHtyp U V (or_intror _ (refl_equal (Sum U V)))).
+  simpl in t0 ; intuition.
+  pose (IHtyp U V (or_intror _ (refl_equal (Sum U V)))).
+  simpl in t0 ; intuition.
+    
+  induction M ; intuition ; try discriminate.
+  generalize H4 ; unfold subst, subst_rec.
   elim (lt_eq_lt_dec 0 n) ; intros a ; try discriminate.
   case a ; clear a ; intros ; try discriminate.
-  rewrite lift0 in H4.
-  rewrite H4 in H.
-  pose (prod_arity_not_kind H) ; auto with coc.
+  rewrite lift0. rewrite lift0 in H3.
+  rewrite H3 ; rewrite H3 in H.
+  pose (type_has_no_kind H) ; auto with coc.
   
   intros ; discriminate.
-  pose (prod_arity_not_kind H2).
-  simpl in n.
+  pose (type_has_no_kind H2).
+  pose (type_has_no_kind H).
+  unfold subst ; apply type_range_subst_not_kind ; auto.
   
-  unfold subst in H3 ; simpl in H3.
-  inversion H3.
-  pose (prod_arity_not_kind H).
-  apply prod_subst_to_sort ; auto.
+  unfold subst in H4 ; simpl in H4.
+  inversion H4.
+  pose (type_has_no_kind H2).
+  pose (type_has_no_kind H).
+  unfold subst ; apply type_range_subst_not_kind ; auto.
 
-  Focus 3.
-  rewrite H2 in H0.
-  apply (prod_arity_not_kind H0).
+  unfold subst in H4 ; simpl in H4.
+  inversion H4.
+  pose (type_has_no_kind H2).
+  pose (type_has_no_kind H).
+  unfold subst ; apply type_range_subst_not_kind ; auto.
+  
+  destruct H2 ;
+  rewrite H2 in H0 ;
+  rewrite H2 ; apply (type_has_no_kind H0).
 
-  Focus 3.
   destruct H.
-  elim (inv_nth_nl _ _ _ H0).
+  elim (inv_nth_nl _ _ _ H1).
   
-  Focus 3.
   assert (wf (T :: e)). 
   apply wf_var with s ; auto with coc.
-  destruct (wf_sort_lift _ (T :: e) _ H1 H0).
-  apply (prod_arity_not_kind H2).
+  destruct (wf_sort_lift _ (T :: e) _ H2 H0).
+  apply (type_has_no_kind H3).
+Qed.
 
-
-Lemma prod_target_not_kindtype : forall t G T, G |- t : T -> 
-  forall U V, T = Prod U V -> ~ (exists n, prod_target T n (Srt kind)).
+Lemma type_no_kind_prod_type : forall G t U V, 
+  G |- t : Prod U V -> type_no_kind V.
 Proof.
-induction T ; try solve [unfold prod_sort ; red ; intros ; try discriminate].
-intros.
-induction (prod_dec V).
-induction a.
-induction H1.
-red ; intros.
-rewrite H0 in H2.
-simpl in H2.
-injection H0.
-intros.
-rewrite H3 in IHT2.
+  intros.
+  pose (type_no_kind_type H (or_introl _ (refl_equal (Prod U V)))).
+  simpl in t0.
+  intuition.
+Qed.
 
-induction H ; try discriminate.
+Lemma type_no_kind_prod_type2 : forall G t U V, 
+  G |- t : Prod U V -> type_no_kind (Prod U V).
+Proof.
+  intros.
+  pose (type_no_kind_type H (or_introl _ (refl_equal (Prod U V)))).
+  simpl in t0.
+  intuition.
+  simpl ; auto.
+Qed.
 
-injection H0 ; intros.
-rewrite H6 in H5.
-apply (IHT2 _ _ H5 _ _ H1).
-induction H2.
-inversion H2.
-pose (inv_lift_sort T0 1 H12).
-rewrite e0 in H11.
-exists n ; rewrite H12 ; apply H11.
+Lemma type_no_kind_prod_type_sort : forall G t U V, 
+  G |- t : Prod U V -> 
+  forall s, type_range V = Srt s -> s <> kind.
+Admitted.
 
-apply (IHtyp1 H0).
-
-injection H0 ; intros.
-rewrite H1 in IHt2.
-induction H ; try discriminate.
-injection H0 ; intros.
-rewrite H4 in H3.
-
-red ; intros.
-
-simpl in H6.
-rewrite H4 in H6.
-induction H6.
-inversion H6.
-pose (inv_lift_sort T0 1 H11).
-induction V ; try solve [
-  inversion H10 ; rewrite H15 in H3 ; rewrite e0 in H3 ; apply (typ_not_kind H3) ; auto ].
-clear IHV1 ; clear IHV2.
-
-apply (b V1 V2) ; auto.
-
-apply IHtyp1 ; auto.
-
-
+Lemma type_no_kind_sum_type : forall G t U V, 
+  G |- t : Sum U V -> type_no_kind V.
+Proof.
+  intros.
+  pose (type_no_kind_type H (or_intror _ (refl_equal (Sum U V)))).
+  simpl in t0.
+  intuition.
+Qed.
 
 Definition is_low_sort (s : term) := s = Srt set \/ s = Srt prop.
 
@@ -368,7 +329,7 @@ Proof.
 Qed.
 
 Lemma kind_is_prod : forall G t T, G |- t : T -> T = Srt kind ->
-  is_low_sort (prod_sort t).
+  is_low_sort (type_range t).
 Proof.
   induction 1 ; intros ; try discriminate ; simpl ; auto.
   unfold is_low_sort ; intuition.
@@ -379,148 +340,1382 @@ Proof.
   
   pose (subst_to_sort _ H1 (typ_not_kind H)).
 
-  pose (prod_target_not_kind). H0) . (refl_equal (Prod V Ur))).
-  
+  pose (type_no_kind_type H0 (or_introl _ (refl_equal (Prod V Ur)))).
+  simpl in t.
+  destruct t.
+  rewrite e0 in H3.
+  simpl in H3.
+  contradiction.
 
+  pose (type_no_kind_type H (or_intror _ (refl_equal (Sum U V)))).
+  simpl in t0.
+  destruct t0.
+  rewrite H0 in H1.
+  simpl in H1.
+  contradiction.
 
-  pose (typ_sort H).
+  pose (type_no_kind_type H (or_intror _ (refl_equal (Sum U V)))).
+  simpl in t0.
+  destruct t0.
+  assert(Pi1 t <> Srt kind) ; try (unfold not ; intros ; discriminate).
+  pose (subst_to_sort _ H0 H3).
+  rewrite e0 in H2.
+  simpl in H2.
+  contradiction.
 
-typ_lift_sort).
+  pose (type_has_no_kind H).
+  pose (type_has_no_kind H2).
+  unfold subst in H3.
+  pose (type_range_subst_not_kind _ _ 0 t0 t1).
+  pose (type_no_kind_not_kind t2).
+  contradiction.
 
+  rewrite H3 in H0.
+  pose (typ_not_kind H0).
+  elim n ; auto.
+Qed.
 
-(*
-Lemma prod_target_dec : forall T U, {exists n, prod_target T n U} + {forall n, ~ prod_target T n U}.
+Lemma red_sort_eq : forall s t, red (Srt s) t -> t = Srt s.
+Proof.
+  simple induction 1; intros; auto with coc core arith sets.
+  rewrite H1 in H2.
+  inversion H2.
+Qed.
+
+Lemma sort_conv_eq : forall G T s, G |- T : Srt kind -> conv T (Srt s) -> T = Srt s.
 Proof.
   intros.
-  set (Tfull := T).
-  induction T ; 
-  (induction (eqterm Tfull U) as [a | a] ; [
-  (left ; exists 0 ; rewrite <- a ;
-  unfold Tfull ; eapply prod_target_0 ; auto ; red ; intros ; try discriminate) |
-  (right ; intros ; red ; intros ; inversion H ; try contradiction) ]).
+  destruct (church_rosser _ _ H0).
+  pose (red_sort_eq H2).
+  rewrite e in H1.
+
+  pose (kind_is_prod H (refl_equal (Srt kind))).
+  unfold is_low_sort in i.
+  induction T ; try (simpl in i ; destruct i ; inversion H1 ; try discriminate) ; auto with coc core.
+
+  rewrite (conv_sort _ _ H0).
+  auto.
+
+  rewrite (conv_sort _ _ H0).
+  auto.
+
+  pose (conv_sort_prod s T1 T2).
+  pose (sym_conv _ _ H0).
+  contradiction.
+
+  pose (conv_sort_prod s T1 T2).
+  pose (sym_conv _ _ H0).
+  contradiction.
+
+  pose (conv_sort_sum s T1 T2).
+  pose (sym_conv _ _ H0).
+  contradiction.
+
+  pose (conv_sort_sum s T1 T2).
+  pose (sym_conv _ _ H0).
+  contradiction.
+Qed.
+
+Lemma coerce_prop_sort_l_aux : forall G Ts A s', G |- Ts >> A : s' ->
+  Ts = Srt prop ->  s' = kind -> G |- A : Srt kind -> A = Srt prop.
+Proof.
+  induction 1 ; simpl ; intros ; try discriminate.
+  apply sort_conv_eq with e ; auto.
+  rewrite H2 in H1 ; auto with coc.
+
+  apply IHcoerce2 ; auto.
+  apply IHcoerce1 ; auto.
+  rewrite H2 in H0.
+  apply coerce_sort_l with C ; auto.
+Qed.
+
+Lemma coerce_set_sort_l_aux : forall G Ts A s', G |- Ts >> A : s' ->
+  Ts = Srt set ->  s' = kind -> G |- A : Srt kind -> A = Srt set.
+Proof.
+  induction 1 ; simpl ; intros ; try discriminate.
+  apply sort_conv_eq with e ; auto.
+  rewrite H2 in H1 ; auto with coc.
+
+  apply IHcoerce2 ; auto.
+  apply IHcoerce1 ; auto.
+  rewrite H2 in H0.
+  apply coerce_sort_l with C ; auto.
+Qed.
+
+
+Lemma coerce_prop_sort_r_aux : forall G Ts A s', G |- A >> Ts : s' ->
+  Ts = Srt prop ->  s' = kind -> G |- A : Srt kind -> A = Srt prop.
+Proof.
+  induction 1 ; simpl ; intros ; try discriminate.
+  apply sort_conv_eq with e ; auto.
+  rewrite H2 in H1 ; auto with coc.
+
+  apply IHcoerce1 ; auto.
+  apply IHcoerce2 ; auto.
+  rewrite H2 in H0.
+  apply coerce_sort_l with C ; auto.
+Qed.
+
+Lemma coerce_set_sort_r_aux : forall G Ts A s', G |- A >> Ts : s' ->
+  Ts = Srt set ->  s' = kind -> G |- A : Srt kind -> A = Srt set.
+Proof.
+  induction 1 ; simpl ; intros ; try discriminate.
+  apply sort_conv_eq with e ; auto.
+  rewrite H2 in H1 ; auto with coc.
+
+  apply IHcoerce1 ; auto.
+  apply IHcoerce2 ; auto.
+  rewrite H2 in H0.
+  apply coerce_sort_l with C ; auto.
+Qed.
+
+Lemma coerce_prop_sort_l : forall G A, G |- Srt prop >> A : kind -> A = Srt prop.
+Proof. 
+  intros.
+  eapply coerce_prop_sort_l_aux with G (Srt prop) kind ; auto.
+  apply coerce_sort_r with (Srt prop) ; auto.
+Qed.
+
+Lemma coerce_prop_sort_r : forall G A, G |- A >> Srt prop : kind -> A = Srt prop.
+Proof. 
+  intros.
+  eapply coerce_prop_sort_r_aux with G (Srt prop) kind ; auto.
+  apply coerce_sort_l with (Srt prop) ; auto.
+Qed.
+
+Lemma coerce_set_sort_l : forall G A, G |- Srt set >> A : kind -> A = Srt set.
+Proof. 
+  intros.
+  eapply coerce_set_sort_l_aux with G (Srt set) kind ; auto.
+  apply coerce_sort_r with (Srt set) ; auto.
+Qed.
+
+Lemma coerce_set_sort_r : forall G A, G |- A >> Srt set : kind -> A = Srt set.
+Proof. 
+  intros.
+  eapply coerce_set_sort_r_aux with G (Srt set) kind ; auto.
+  apply coerce_sort_l with (Srt set) ; auto.
+Qed.
+
+Lemma coerce_propset_l : forall G A s s', G |- Srt s >> A : s' -> A = Srt s.
+Proof.
+  intros.
+  assert(s' = kind).
+  pose (coerce_sort_l _ _ _ _ H).
+  pose (typ_sort _ _ _ t).
+  intuition.
+  inversion H1 ; auto.
+  rewrite H0 in H.
+  clear H0.
+  induction s.
+  pose (coerce_sort_l _ _ _  _ H).
+  pose (typ_not_kind t).
+  elim n ; auto.
+  
+  eapply coerce_prop_sort_l with G ; auto with coc.
+  eapply coerce_set_sort_l with G ; auto with coc.
+Qed.
+
+Lemma coerce_propset_r : forall G A s s', G |- A >> Srt s : s' -> A = Srt s.
+Proof.
+  intros.
+  assert(s' = kind).
+  pose (coerce_sort_r _ _ _ _ H).
+  pose (typ_sort _ _ _ t).
+  intuition.
+  inversion H1 ; auto.
+  rewrite H0 in H.
+  clear H0.
+  induction s.
+  pose (coerce_sort_r _ _ _  _ H).
+  pose (typ_not_kind t).
+  elim n ; auto.
+  
+  eapply coerce_prop_sort_r with G ; auto with coc.
+  eapply coerce_set_sort_r with G ; auto with coc.
+Qed.
+
+
+Lemma wf_is_sorted : forall e, wf e ->
+  forall x n, item _ x e n -> forall s, x = Srt s -> is_prop s.
+Proof.
+  induction 1 ; simpl ; intros ; auto with coc.
+  elim (inv_nth_nl _ _ _ H).
+  pose (item_trunc).
+  induction (item_trunc _ _ _ _ H0).
+
+  pose (wf_sort).
+  pose (wf_var _ _ _ H).
+  induction (wf_sort n _ _ H2 w x H0).
+  rewrite H1 in H3.
+  pose (typ_sort _ _ _ H3).
+  intuition.
+Qed.
+
+
+Lemma inv_lift_sort : forall t s n, lift n t = Srt s -> t = Srt s.
+Proof.
+intros.
+induction t ; simpl ; try discriminate.
+unfold lift in H ; simpl in H.
+auto.
+Qed.
+
+Lemma gen_sorting_var_aux : forall e t T, e |- t : T ->
+  forall n, t = Ref n -> 
+  forall s, T = (Srt s) ->
+  is_prop s.
+Proof.
+  induction 1 using typ_mutwf with
+   (P := fun e t T => fun H : e |- t : T =>
+   forall n, t = Ref n -> 
+   forall s, T = (Srt s) ->
+   is_prop s)
+   (P0 := fun e T U s => fun H : e |- T >> U : s =>
+   True)
+   (P1 := fun e => fun H : wf e =>
+   forall s, forall n, item _ (Srt s) e n -> is_prop s)
+ ; try (simpl ; intros ; try discriminate ; auto with coc).
+ 
+  rewrite H0 in i.
+  destruct i.
+  rewrite (inv_lift_sort x (S n) (sym_eq H1)) in H2.
+  apply (IHtyp s n).
+  auto.
+ 
+  rewrite H3 in H0.
+  pose (typ_sort _ _ _ H0).
+  intuition.
+ 
+  elim (inv_nth_nl _ _ _ H).
+
+  pose (wf_is_sorted).
+  apply wf_is_sorted with (T :: e) (Srt s0) n ; auto with coc.
+  eapply wf_var with s ; auto with coc.
+Qed.
+
+Lemma gen_sorting_var : 
+  forall e n s, e |- Ref n : Srt s -> is_prop s.
+Proof.
+  intros.
+  apply gen_sorting_var_aux with e (Ref n) (Srt s) n ; auto.
+Qed.
+
+Lemma gen_sorting_app_aux : forall e t Ts, e |- t : Ts ->
+  forall M N, t = App M N ->
+  forall s, Ts = Srt s -> is_prop s.
+Proof.
+  induction 1 ; simpl ; intros ; try discriminate.
+
+  inversion_clear H1.
+  pose (type_no_kind_prod_type H0).
+  induction s ; unfold is_prop ; simpl ; auto.
+  pose (subst_to_sort _ H2 (typ_not_kind H)).
+  rewrite e0 in t.
+  simpl in t ; contradiction.
+
+  rewrite H4 in H0.
+  pose (typ_sort _ _ _ H0).
+  intuition.
+Qed.
+
+Lemma gen_sorting_app : forall e M N s, e |- App M N : Srt s -> is_prop s.
+Proof.
+  intros.
+  eapply gen_sorting_app_aux with e (App M N) (Srt s) M N ; auto ; auto.
+Qed.
+
+Lemma sorting_lambda_aux : forall e t Ts, e |- t : Ts ->
+  forall T M, t = Abs T M -> forall s, Ts <> Srt s.
+Proof.
+  induction 1 ; simpl ; intros ; try discriminate.
+  unfold not ; intros.
+  rewrite H4 in H0.
+  destruct (typ_sort _ _ _ H0).
+  inversion H6.
+  rewrite H8 in H2.
+  rewrite H4 in H2.
+  pose (coerce_propset_r H2).
+  pose (IHtyp1 T M H3 s0).
+  contradiction.
+Qed.
+(*
+Lemma sorting_lambda_range_aux : forall e t Ts, e |- t : Ts ->
+  forall T M, t = Abs T M -> forall s, type_range Ts <> Srt s.
+Proof.
+  induction 1 ; simpl ; intros ; try discriminate.
+  unfold not ; intros.
+
+  induction U ; simpl ; intros ; try discriminate.
+  simpl in H3.
+  assert(e |- Abs T M : Prod T (Srt s0)).
+  apply type_abs with s1 s2 ; auto.
+  pose (sorting_lambda_aux 
+
+
+
+  destruct (typ_sort _ _ _ H0).
   
 
-  induction IHT2.
+  rewrite H4 in H0.
+  destruct (typ_sort _ _ _ H0).
+  inversion H6.
+  rewrite H8 in H2.
+  rewrite H4 in H2.
+  pose (coerce_propset_r H2).
+  pose (IHtyp1 T M H3 s0).
+  contradiction.
+Qed.
+*)
+Lemma sorting_lambda : forall e T M s, ~ e |- Abs T M : Srt s.
+Proof.
+  unfold not ; intros.
+  apply (sorting_lambda_aux H (refl_equal (Abs T M)) (refl_equal (Srt s))).
+Qed.
+
+Lemma generation_prod_aux : forall e T Ts, e |- T : Ts ->
+  forall U V, T = Prod U V -> exists s, Ts = Srt s.
+Proof.
+  induction 1 ; simpl ; intros ; try discriminate.
+  exists s2 ; auto.
+
+  destruct (IHtyp1 U0 V0 H3).
+  rewrite H4 in H1.
+  induction (typ_sort _ _ _ H1).
+  inversion H6.
+  rewrite H8 in H2.
+  rewrite H4 in H2.
+  pose (coerce_propset_l H2).
+  exists x ; auto.
+Qed.
+
+Lemma generation_prod : forall e U V Ts, e |- Prod U V : Ts ->
+  exists s, Ts = Srt s.
+Proof.
+  intros.
+  eapply generation_prod_aux with e (Prod U V) U V ; auto.
+Qed.
+
+Lemma generation_prod2_aux : forall e T Ts, e |- T : Ts ->
+  forall U V, T = Prod U V -> forall s, Ts = Srt s ->
+  (exists s', e |- U : Srt s') /\ (U :: e) |- V : Srt s.
+Proof.
+  induction 1 ; simpl ; intros ; try discriminate.
+
+  inversion H1.
+  rewrite H4 in H.
+  rewrite H5 in H0.
+  rewrite H4 in H0.
+
+  split.
+  exists s1 ; auto.
+  inversion H2.
+  rewrite <- H6.
+  assumption.
+
+  rewrite H4 in H2.
+  rewrite H4 in H0.
+  induction (typ_sort _ _  _ H0).
+  inversion H6.
+  rewrite H8 in H2.
+  pose (coerce_propset_r H2).
+
+  apply (IHtyp1 U0 V0 H3 s0 e0).
+Qed.
+
+Lemma generation_prod2 : forall e U V s, e |- Prod U V : Srt s ->
+  (exists s', e |- U : Srt s') /\ (U :: e) |- V : Srt s.
+Proof.
+  intros.
+  eapply generation_prod2_aux  ; auto ; auto.
+Qed.
+
+Lemma generation_sum_aux : forall e T Ts, e |- T : Ts ->
+  forall U V, T = Sum U V -> exists s, Ts = Srt s.
+Proof.
+  induction 1 ; simpl ; intros ; try discriminate.
+  exists s2 ; auto.
+
+  destruct (IHtyp1 U0 V0 H3).
+  rewrite H4 in H1.
+  induction (typ_sort _ _ _ H1).
+  inversion H6.
+  rewrite H8 in H2.
+  rewrite H4 in H2.
+  pose (coerce_propset_l H2).
+  exists x ; auto.
+Qed.
+
+Lemma generation_sum : forall e U V Ts, e |- Sum U V : Ts ->
+  exists s, Ts = Srt s.
+Proof.
+  intros.
+  eapply generation_sum_aux with e (Sum U V) U V ; auto.
+Qed.
+
+Lemma generation_sum2_aux : forall e T Ts, e |- T : Ts ->
+  forall U V, T = Sum U V -> forall s, Ts = Srt s ->
+  (exists s', e |- U : Srt s') /\ (U :: e) |- V : Srt s.
+Proof.
+  induction 1 ; simpl ; intros ; try discriminate.
+
+  inversion H1.
+  rewrite H4 in H.
+  rewrite H5 in H0.
+  rewrite H4 in H0.
+
+  split.
+  exists s1 ; auto.
+  inversion H2.
+  rewrite <- H6.
+  assumption.
+
+  rewrite H4 in H2.
+  rewrite H4 in H0.
+  induction (typ_sort _ _  _ H0).
+  inversion H6.
+  rewrite H8 in H2.
+  pose (coerce_propset_r H2).
+
+  apply (IHtyp1 U0 V0 H3 s0 e0).
+Qed.
+
+Lemma generation_sum2 : forall e U V s, e |- Sum U V : Srt s ->
+  (exists s', e |- U : Srt s') /\ (U :: e) |- V : Srt s.
+Proof.
+  intros.
+  eapply generation_sum2_aux  ; auto ; auto.
+Qed.
+
+Lemma generation_subset_aux : forall e T Ts, e |- T : Ts ->
+  forall U V, T = Subset U V -> Ts = Srt set.
+Proof.
+  induction 1 ; simpl ; intros ; try discriminate.
+  auto.
+
+  pose (IHtyp1 U0 V0 H3).
+  rewrite e0 in H2.
+  exact (coerce_propset_l H2).
+Qed.
+
+Lemma generation_subset : forall e U V Ts, e |- Subset U V : Ts ->
+  Ts = Srt set.
+Proof.
+  intros.
+  eapply generation_subset_aux with e (Subset U V) U V ; auto.
+Qed.
+
+Lemma generation_subset2_aux : forall e T Ts, e |- T : Ts ->
+  forall U V, T = Subset U V -> Ts = Srt set ->
+  e |- U : Srt set /\ (U :: e) |- V : Srt prop.
+Proof.
+  induction 1 ; simpl ; intros ; try discriminate.
+
+  inversion H1.
+  rewrite H4 in H.
+  rewrite H5 in H0.
+  rewrite H4 in H0.
+  intuition.
+
+  rewrite H4 in H2.
+  pose (coerce_propset_r H2).
+ 
+  apply (IHtyp1 U0 V0 H3 e0).
+Qed.
+
+Lemma generation_subset2 : forall e U V s, e |- Subset U V : Srt set ->
+  (e |- U : Srt set) /\ (U :: e) |- V : Srt prop.
+Proof.
+  intros.
+  eapply generation_subset2_aux  ; auto ; auto.
+Qed.
+
+Lemma var_sort_item : forall e t T, e |- t : T ->
+  forall n, t = Ref n -> 
+  forall s, T = (Srt s) -> item _ (Srt s) e n.
+Proof.
+  induction 1 ; simpl ; intros ; try discriminate ; auto with coc.
+  inversion H1.
+
+  rewrite H2 in H0.
+  rewrite <- H4 ; auto.
+  destruct H0.
+  assert(x = Srt s).
+  apply (inv_lift_sort) with (S n) ; auto.
+  rewrite H5 in H3 ; assumption.
+
+  rewrite H4 in H2.
+  pose (coerce_propset_r H2).
+  pose (IHtyp1 n H3 s0 e0).
+  assumption.
+Qed. 
+
+Lemma conv_is_low_range : forall A s, conv (Srt s) A -> is_low_sort (type_range A) -> A = Srt s.
+Proof.
+  induction A ; simpl ; intros ; 
+  try unfold is_low_sort in H0 ; intuition ; try discriminate ; auto with coc core datatypes.
+  
+  rewrite (conv_sort _ _ H).
+  auto.
+
+  rewrite (conv_sort _ _ H).
+  auto.
+
+  elim conv_sort_prod with s A1 A2 ; auto with coc core.
+  elim conv_sort_prod with s A1 A2 ; auto with coc core.
+
+  elim conv_sort_sum with s A1 A2 ; auto with coc core.
+  elim conv_sort_sum with s A1 A2 ; auto with coc core.
+Qed.
+
+Lemma conv_is_low_dom : forall A s, conv (Srt s) A -> 
+  is_low_sort (type_dom A) -> A = Srt s.
+Proof.
+  induction A ; simpl ; intros ; 
+  try unfold is_low_sort in H0 ; intuition ; try discriminate ; auto with coc core datatypes.
+  
+  rewrite (conv_sort _ _ H).
+  auto.
+
+  rewrite (conv_sort _ _ H).
+  auto.
+
+  elim conv_sort_prod with s A1 A2 ; auto with coc core.
+  elim conv_sort_prod with s A1 A2 ; auto with coc core.
+
+  elim conv_sort_sum with s A1 A2 ; auto with coc core.
+  elim conv_sort_sum with s A1 A2 ; auto with coc core.
+Qed.
+
+Lemma conv_is_low_range_full : forall A B, conv A B ->
+  is_low_sort (type_range A) -> 
+  is_low_sort (type_range B) -> type_range A = type_range B.
+Proof.
+  induction A ; simpl ; intros ; 
+  try unfold is_low_sort in H0 ;   
+  intuition ; try discriminate ; auto with coc core datatypes.
+  
+  rewrite (conv_is_low_range H H1).
+  simpl ; auto.
+
+  rewrite (conv_is_low_range H H1).
+  simpl ; auto.
+  
+  induction B ; simpl ; intros ; 
+  try unfold is_low_sort in H1 ;   
+  intuition ; try discriminate ; auto with coc core datatypes.
+
+  elim conv_sort_prod with s A1 A2 ; auto with coc core.
+  elim conv_sort_prod with s A1 A2 ; auto with coc core.
+
+  simpl in H0.
+  apply (IHA2 B2 (inv_conv_prod_r _ _ _ _ H)).
+  unfold is_low_sort ; rewrite H2 ; auto.
+  unfold is_low_sort ; rewrite H0 ; auto.
+
+  simpl in H0.
+  apply (IHA2 B2 (inv_conv_prod_r _ _ _ _ H)).
+  unfold is_low_sort ; rewrite H2 ; auto.
+  unfold is_low_sort ; rewrite H0 ; auto.
+
+  elim conv_prod_sum with A1 A2 B1 B2 ; auto with coc.
+  elim conv_prod_sum with A1 A2 B1 B2 ; auto with coc.
+
+  induction B ; simpl ; intros ; 
+  try unfold is_low_sort in H1 ;   
+  intuition ; try discriminate ; auto with coc core datatypes.
+
+  elim conv_sort_prod with s A1 A2 ; auto with coc core.
+  elim conv_sort_prod with s A1 A2 ; auto with coc core.
+
+  simpl in H0.
+  apply (IHA2 B2 (inv_conv_prod_r _ _ _ _ H)).
+  unfold is_low_sort ; rewrite H2 ; auto.
+  unfold is_low_sort ; rewrite H0 ; auto.
+
+  simpl in H0.
+  apply (IHA2 B2 (inv_conv_prod_r _ _ _ _ H)).
+  unfold is_low_sort ; rewrite H2 ; auto.
+  unfold is_low_sort ; rewrite H0 ; auto.
+
+  elim conv_prod_sum with A1 A2 B1 B2 ; auto with coc.
+  elim conv_prod_sum with A1 A2 B1 B2 ; auto with coc.
+
+  induction B ; simpl ; intros ; 
+  try unfold is_low_sort in H1 ;   
+  intuition ; try discriminate ; auto with coc core datatypes.
+
+  elim conv_sort_sum with s A1 A2 ; auto with coc core.
+  elim conv_sort_sum with s A1 A2 ; auto with coc core.
+
+  elim conv_prod_sum with B1 B2 A1 A2; auto with coc core.
+  elim conv_prod_sum with B1 B2 A1 A2; auto with coc core.
+
+  simpl in H0.
+  apply (IHA2 B2 (inv_conv_sum_r _ _ _ _ H)).
+  unfold is_low_sort ; rewrite H2 ; auto.
+  unfold is_low_sort ; rewrite H0 ; auto.
+
+  simpl in H0.
+  apply (IHA2 B2 (inv_conv_sum_r _ _ _ _ H)).
+  unfold is_low_sort ; rewrite H2 ; auto.
+  unfold is_low_sort ; rewrite H0 ; auto.
+
+  induction B ; simpl ; intros ; 
+  try unfold is_low_sort in H1 ;   
+  intuition ; try discriminate ; auto with coc core datatypes.
+
+  elim conv_sort_sum with s A1 A2 ; auto with coc core.
+  elim conv_sort_sum with s A1 A2 ; auto with coc core.
+
+  elim conv_prod_sum with B1 B2 A1 A2; auto with coc core.
+  elim conv_prod_sum with B1 B2 A1 A2; auto with coc core.
+
+  simpl in H0.
+  apply (IHA2 B2 (inv_conv_sum_r _ _ _ _ H)).
+  unfold is_low_sort ; rewrite H2 ; auto.
+  unfold is_low_sort ; rewrite H0 ; auto.
+
+  simpl in H0.
+  apply (IHA2 B2 (inv_conv_sum_r _ _ _ _ H)).
+  unfold is_low_sort ; rewrite H2 ; auto.
+  unfold is_low_sort ; rewrite H0 ; auto.
+Qed.
+
+Lemma conv_is_low_dom_full : forall A B, conv A B ->
+  is_low_sort (type_dom A) -> 
+  is_low_sort (type_dom B) -> type_dom A = type_dom B.
+Proof.
+  induction A ; simpl ; intros ; 
+  try unfold is_low_sort in H0 ;   
+  intuition ; try discriminate ; auto with coc core datatypes.
+  
+  rewrite (conv_is_low_dom H H1).
+  simpl ; auto.
+
+  rewrite (conv_is_low_dom H H1).
+  simpl ; auto.
+  
+  induction B ; simpl ; intros ; 
+  try unfold is_low_sort in H1 ;   
+  intuition ; try discriminate ; auto with coc core datatypes.
+
+  elim conv_sort_prod with s A1 A2 ; auto with coc core.
+  elim conv_sort_prod with s A1 A2 ; auto with coc core.
+
+  simpl in H0.
+  rewrite H0 ; rewrite H2 ; auto.
+  
+  simpl in H0.
+  pose (IHA1 B1 (inv_conv_prod_l _ _ _ _ H)).
+  unfold is_low_sort ; rewrite H2 ; auto.
+  unfold is_low_sort ; rewrite H0 ; auto.
+
+  simpl in H0.
+  apply (IHA1 B1 (inv_conv_prod_l _ _ _ _ H)).
+  unfold is_low_sort ; rewrite H2 ; auto.
+  unfold is_low_sort ; rewrite H0 ; auto.
+
+  elim conv_prod_sum with A1 A2 B1 B2 ; auto with coc.
+  elim conv_prod_sum with A1 A2 B1 B2 ; auto with coc.
+
+  induction B ; simpl ; intros ; 
+  try unfold is_low_sort in H1 ;   
+  intuition ; try discriminate ; auto with coc core datatypes.
+
+  elim conv_sort_prod with s A1 A2 ; auto with coc core.
+  elim conv_sort_prod with s A1 A2 ; auto with coc core.
+
+  simpl in H0.
+  apply (IHA2 B2 (inv_conv_prod_r _ _ _ _ H)).
+  unfold is_low_sort ; rewrite H2 ; auto.
+  unfold is_low_sort ; rewrite H0 ; auto.
+
+  simpl in H0.
+  apply (IHA2 B2 (inv_conv_prod_r _ _ _ _ H)).
+  unfold is_low_sort ; rewrite H2 ; auto.
+  unfold is_low_sort ; rewrite H0 ; auto.
+
+  elim conv_prod_sum with A1 A2 B1 B2 ; auto with coc.
+  elim conv_prod_sum with A1 A2 B1 B2 ; auto with coc.
+
+  induction B ; simpl ; intros ; 
+  try unfold is_low_sort in H1 ;   
+  intuition ; try discriminate ; auto with coc core datatypes.
+
+  elim conv_sort_sum with s A1 A2 ; auto with coc core.
+  elim conv_sort_sum with s A1 A2 ; auto with coc core.
+
+  elim conv_prod_sum with B1 B2 A1 A2; auto with coc core.
+  elim conv_prod_sum with B1 B2 A1 A2; auto with coc core.
+
+  simpl in H0.
+  apply (IHA2 B2 (inv_conv_sum_r _ _ _ _ H)).
+  unfold is_low_sort ; rewrite H2 ; auto.
+  unfold is_low_sort ; rewrite H0 ; auto.
+
+  simpl in H0.
+  apply (IHA2 B2 (inv_conv_sum_r _ _ _ _ H)).
+  unfold is_low_sort ; rewrite H2 ; auto.
+  unfold is_low_sort ; rewrite H0 ; auto.
+
+  induction B ; simpl ; intros ; 
+  try unfold is_low_sort in H1 ;   
+  intuition ; try discriminate ; auto with coc core datatypes.
+
+  elim conv_sort_sum with s A1 A2 ; auto with coc core.
+  elim conv_sort_sum with s A1 A2 ; auto with coc core.
+
+  elim conv_prod_sum with B1 B2 A1 A2; auto with coc core.
+  elim conv_prod_sum with B1 B2 A1 A2; auto with coc core.
+
+  simpl in H0.
+  apply (IHA2 B2 (inv_conv_sum_r _ _ _ _ H)).
+  unfold is_low_sort ; rewrite H2 ; auto.
+  unfold is_low_sort ; rewrite H0 ; auto.
+
+  simpl in H0.
+  apply (IHA2 B2 (inv_conv_sum_r _ _ _ _ H)).
+  unfold is_low_sort ; rewrite H2 ; auto.
+  unfold is_low_sort ; rewrite H0 ; auto.
+Qed.
+
+Lemma term_type_range_kinded : forall e t T, e |- t : T ->
+  forall s, type_range t = Srt s -> T = Srt kind. 
+Proof.
+  induction 1 ; simpl ; intros ; try discriminate ; auto with coc.
+  
+  apply IHtyp2 with s ; auto.
+  apply IHtyp2 with s ; auto.
+  
+  rewrite (IHtyp1 _ H3) in H1.
+  elim typ_not_kind2 with e (Srt s) ; auto.
+Qed.
+
+Lemma type_range_sub : forall e T U s, e |- T >> U : s ->
+  forall s0, type_range U = Srt s0 -> type_range T = Srt s0.
+Proof.
+  induction 1 ; simpl ; intros ; try discriminate ; auto with coc.
+  induction B ; try discriminate.
+  simpl in H2.
+  inversion H2.
+  induction (typ_sort _ _ _ H0).
+  inversion H5.
+  rewrite H7 in H.
+  pose (kind_is_prod H (refl_equal (Srt kind))).
+  rewrite (conv_is_low_range (sym_conv _ _ H1) i).
+  simpl ; assumption.
+
+  rewrite <- H2.
+  pose (term_type_range_kinded H0 H2).
+  inversion e0.
+  rewrite H4 in H0.
+  
+  apply (conv_is_low_range_full H1).
+  apply kind_is_prod with e (Srt s) ; auto.
+  apply kind_is_prod with e (Srt s) ; auto.
+
+  rewrite <- H2.
+  pose (term_type_range_kinded H0 H2).
+  inversion e0.
+  rewrite H4 in H0.
+  
+  apply (conv_is_low_range_full H1).
+  apply kind_is_prod with e (Srt s) ; auto.
+  apply kind_is_prod with e (Srt s) ; auto.
+
+  pose (coerce_sort_r _ _ _ _ H).
+  pose (term_type_range_kinded t H1).
+  discriminate.
+Qed.
+
+Lemma type_dom_sub : forall e T U s, e |- T >> U : s ->
+  forall s0, type_dom U = Srt s0 -> type_dom T = Srt s0.
+Proof.
+  induction 1 ; simpl ; intros ; try discriminate ; auto with coc.
+  induction B ; try discriminate.
+  simpl in H2.
+  inversion H2.
+  induction (typ_sort _ _ _ H0).
+  inversion H5.
+  rewrite H7 in H.
+  pose (kind_is_prod H (refl_equal (Srt kind))).
+  rewrite (conv_is_low_range (sym_conv _ _ H1) i).
+  simpl ; assumption.
+
+  rewrite <- H2.
+  simpl in H2.
+  destruct (generation_prod2 H0).
+  induction H3.
+  pose (term_type_range_kinded H3 H2).
+  inversion e0.
+  rewrite H6 in H3.
+  
+  
+  apply (conv_is_low_range_full H1).
+  apply kind_is_prod with e (Srt s) ; auto.
+  apply kind_is_prod with e (Srt s) ; auto.
+
+  rewrite <- H2.
+  pose (term_type_range_kinded H0 H2).
+  inversion e0.
+  rewrite H4 in H0.
+  
+  apply (conv_is_low_range_full H1).
+  apply kind_is_prod with e (Srt s) ; auto.
+  apply kind_is_prod with e (Srt s) ; auto.
+
+  pose (coerce_sort_r _ _ _ _ H).
+  pose (term_type_range_kinded t H1).
+  discriminate.
+Qed.
+
+
+Lemma var_sort_range_item_aux : forall e t T, e |- t : T ->
+  forall n, t = Ref n -> 
+  forall s, type_range T = (Srt s) -> 
+  exists T', item_lift T' e n /\ type_range T' = Srt s.
+Proof.
+  induction 1 ; simpl ; intros ; try discriminate ; auto with coc.
+  inversion H1.
+  
+  induction T ; simpl ; simpl in H2 ; try discriminate.
+  
+  rewrite H2 in H0.
+  rewrite <- H4 ; auto.
+  destruct H0.
+  assert(x = Srt s).
+  apply (inv_lift_sort) with (S n) ; auto.
+  inversion H2.
+  exists (Srt s).
+  simpl ; intuition ; auto.
+  exists (Srt s) ; unfold lift ; simpl ; auto.
+  rewrite H5 in H3 ; assumption.
+  
+  inversion H1.
+  exists (Prod T1 T2).
+  intuition ; auto.
+  rewrite <- H5 ; assumption.
+  
+  inversion H1.
+  exists (Sum T1 T2).
+  intuition ; auto.
+  rewrite <- H5 ; assumption.
+
+  exact (IHtyp1 n H3 s0 (type_range_sub H2 H4)).
+Qed. 
+
+Lemma var_sort_range_item : forall e n T, e |- Ref n : T ->
+  forall s, type_range T = (Srt s) -> 
+  exists T', item_lift T' e n /\ type_range T' = Srt s.
+Proof.
+  intros.
+  eapply var_sort_range_item_aux with (Ref n) T; auto ; auto.
+Qed.
+
+Lemma var_sort_dom_item : forall e n T, e |- Ref n : T ->
+  forall s, type_dom T = (Srt s) -> 
+  exists T', item_lift T' e n /\ type_dom T' = Srt s.
 Admitted.
 
-Lemma prod_subst_aux : forall C n a, 
- forall B, prod_target (subst a C) n B -> 
- (exists k, k < n /\ prod_target C k (Ref k) /\ prod_target a (n - k) B) \/
- (exists B', prod_target C n B' /\ subst a B' = B).
+Lemma unique_var_sort : forall e n s, e |- Ref n : Srt s ->
+  forall s', e |- Ref n : Srt s' -> s = s'.
 Proof.
+  intros.
+  pose (var_sort_item H (refl_equal (Ref n)) (refl_equal (Srt s))).
+  pose (var_sort_item H0 (refl_equal (Ref n)) (refl_equal (Srt s'))).
+  pose (fun_item _ _ _ _ _ i i0).
+  inversion e0 ; auto.
+Qed.
 
-
-Lemma typ_prod_not_kind : forall T G t, G |- t : T -> 
-  forall U V, T = Prod U V -> ~ (exists n, prod_target T n (Srt kind)).
+Lemma unique_var_range_sort : forall e n T, e |- Ref n : T ->
+  forall s, type_range T = Srt s ->
+  forall T', e |- Ref n : T' -> 
+  forall s', type_range T' = Srt s' -> s = s'.
 Proof.
-induction T ; try solve [ intros ; discriminate ].
-induction 1 ; intros ; try discriminate.
-induction (wf_sort_lift _ _ _ H H0).
+  intros.
+  destruct (var_sort_range_item H H0).
+  destruct (var_sort_range_item H1 H2).
+  destruct H3 ; destruct H4.
+  destruct H3 ; destruct H4.
+  pose (fun_item _ _ _ _ _ H7 H8).
+  rewrite <- e0 in H4.
+  rewrite <- H4 in H3.
+  rewrite <- H3 in H6.
+  rewrite H6 in H5.
+  inversion H5.
+  auto.
+Qed.
 
-rewrite H1 in H2.
-pose (prod_target_not_kind H2).
-simpl in n0.
-rewrite H1 ; apply n0 with U V ; auto with coc.
+Lemma unique_var_dom_sort : forall e n T, e |- Ref n : T ->
+  forall s, type_dom T = Srt s ->
+  forall T', e |- Ref n : T' -> 
+  forall s', type_dom T' = Srt s' -> s = s'.
+Proof.
+  intros.
+  destruct (var_sort_dom_item H H0).
+  destruct (var_sort_dom_item H1 H2).
+  destruct H3 ; destruct H4.
+  destruct H3 ; destruct H4.
+  pose (fun_item _ _ _ _ _ H7 H8).
+  rewrite <- e0 in H4.
+  rewrite <- H4 in H3.
+  rewrite <- H3 in H6.
+  rewrite H6 in H5.
+  inversion H5.
+  auto.
+Qed.
 
-injection H2.
-intros.
-rewrite H4 in H.
-rewrite H3 in H0.
-rewrite H4 in H0.
-pose (type_prod _ _ _ H _ _ H0).
-pose (prod_target_not_kind t).
-simpl in n.
-rewrite H2 ; apply n with U0 V ; auto.
+Lemma subst_sort : forall t t' n s, subst_rec t t' n = Srt s -> 
+  t = Srt s \/ t' = Srt s.
+Proof.
+  induction t' ;  simpl ; intros ;
+  auto with coc core arith datatypes ; try discriminate.
+  generalize H.
+  elim (lt_eq_lt_dec n0 n).
+  intros a ; case a ; clear a ; intros ; try discriminate ; auto.
+  left.
+  exact (inv_lift_sort _ _ H0).
 
-red ; intros.
-induction H2.
+  intros.
+  discriminate.
+Qed.
 
-rewrite H1 in H2.
-inversion H2.
-pose (inv_lift_sort T 1 H7).
-rewrite e0 in H6.
-generalize 
-induction n.
-inversion H6.
-rewrite H11 in H1.
-induction Ur ; try solve [unfold subst in H1 ; simpl in H1 ; try discriminate].
+Lemma sort_of_app_aux : forall e t Ts, e |- t : Ts ->
+  forall M N, t = App M N ->
+  forall s, Ts = Srt s ->
+  (exists V, e |- M : Prod V (Srt s)) \/ N = Srt s.
+Proof.
+  induction 1 ; simpl ; intros ;
+  auto with coc core arith datatypes ; try discriminate.
+  inversion H1.
 
-unfold subst in H1.
-generalize H1.
-clear H1.
-unfold subst_rec.
-elim (lt_eq_lt_dec 0 n) ; intros.
-induction a ; try discriminate.
-rewrite lift0 in H1.
-rewrite H1 in H.
-induction (prod_target_not_kind H (refl_equal (Prod U (Srt kind)))).
-exists 1.
-pattern (Srt kind) at 2.
-replace (Srt kind) with (lift 1 (Srt kind)).
-apply prod_target_S.
-apply prod_target_0 with U1 V2 ; auto.
-unfold lift ; simpl ; auto.
-discriminate.
+  induction (subst_sort _ _ _ H2).
+  rewrite <- H5.
+  right ; auto.
+  
+  rewrite H3 in H0.
+  rewrite H4 in H0.
+  left ; exists V ; auto.
 
-unfold subst in H1 ; simpl in H1.
+  rewrite H4 in H2.
+  pose (coerce_propset_r H2).
+  exact (IHtyp1 _ _ H3 _ e0).
+Qed.
 
-apply H10 ; intros.
+Lemma sort_of_app : forall e M N s, e |- App M N : Srt s ->
+  (exists V, e |- M : Prod V (Srt s)) \/ N = Srt s.
+Proof.
+  intros. 
+  eapply sort_of_app_aux ; auto ; auto.
+Qed.
 
-pose (IHtyp2 V Ur (refl_equal (Prod V Ur))).
+Lemma type_range_lift : forall n t k s, type_range (lift_rec n t k) = Srt s -> 
+  type_range t = Srt s.
+Proof.
+  induction t ; simpl ; intros ;
+  auto with coc core arith datatypes ; try discriminate.
+  generalize H ; clear H.
+  elim (le_gt_dec k n0) ;  simpl ; intros ; try discriminate.
+  apply IHt2 with (S k) ; auto.
+  apply IHt2 with (S k) ; auto.
+Qed.
+
+Lemma type_range_subst : forall t u n s, type_range (subst_rec t u n) = Srt s ->
+  type_range t = Srt s \/ type_range u = Srt s.
+Proof.
+  induction u ; simpl ; intros ;
+  auto with coc core arith datatypes ; try discriminate.
+
+  generalize H.
+  elim (lt_eq_lt_dec n0 n) ; simpl ; try (intros ; discriminate).
+  intro a ; case a ; clear a ; simpl ; intros ; try discriminate.
+  unfold lift in H0.
+  left ; exact (type_range_lift _ _ _ H0).
+  
+  apply IHu2 with (S n) ; auto.
+  apply IHu2 with (S n) ; auto.
+Qed.
+
+Lemma sort_of_app_range_aux : forall e t Ts, e |- t : Ts ->
+  forall M N, t = App M N ->
+  forall s, type_range Ts = Srt s ->
+  exists V, exists T,  e |- N : V /\ e |- M : Prod V T /\
+  (type_range T = (Srt s) \/ type_range N = Srt s).
+Proof.
+  induction 1 ; simpl ; intros ;
+  auto with coc core arith datatypes ; try discriminate.
+  inversion H1.
+
+  induction (type_range_subst _ _ _ H2).
+  rewrite <- H5.
+  exists V.
+  exists Ur.
+  rewrite <- H4.
+  split ; auto.
+  
+  exists V ; auto.
+  exists Ur.
+  rewrite <- H5.
+  rewrite <- H4.
+  split ; auto.
+  
+  pose (type_range_sub H2 H4).
+  exact (IHtyp1 _ _ H3 _ e0).
+Qed.
+
+Lemma sort_of_app_range : forall e M N Ts, e |- App M N : Ts ->
+  forall s, type_range Ts = Srt s ->
+  exists V, exists T,  e |- N : V /\ e |- M : Prod V T /\
+  (type_range T = (Srt s) \/ type_range N = Srt s).
+Proof.
+  intros. 
+  apply sort_of_app_range_aux with (App M N) Ts  ; auto ; auto.
+Qed.
+
+Lemma sort_of_abs_range_aux : forall e t Ts, e |- t : Ts ->
+  forall M N, t = Abs M N ->
+  forall s, type_range Ts = Srt s ->
+  exists s1, exists s2, exists T, e |- M : (Srt s1) /\ M :: e |- N : T /\
+  M :: e |- T : Srt s2 /\ type_range T = (Srt s).
+Proof.
+  induction 1 ; simpl ; intros ;
+  auto with coc core arith datatypes ; try discriminate.
+
+  exists s1 ; exists s2.
+  exists U.
+  inversion H2.
+  rewrite <- H5 ; rewrite <- H6.
+  intuition.
+
+  apply (IHtyp1) ; auto.
+  
+  apply (type_range_sub H2 H4).
+Qed.
+
+Lemma sort_of_abs_range : forall e M N Ts, e |- Abs M N : Ts ->
+  forall s, type_range Ts = Srt s ->
+  exists s1, exists s2, exists T, e |- M : (Srt s1) /\ M :: e |- N : T /\
+  M :: e |- T : Srt s2 /\ type_range T = (Srt s).
+Proof.
+  intros. 
+  apply sort_of_abs_range_aux with (Abs M N) Ts  ; auto ; auto.
+Qed.
+
+Lemma sort_of_abs_dom_aux : forall e t Ts, e |- t : Ts ->
+  forall M N, t = Abs M N ->
+  forall s, type_dom Ts = Srt s ->
+  exists s1, exists s2, exists T, e |- M : (Srt s1) /\ M :: e |- N : T /\
+  M :: e |- T : Srt s2 /\ type_dom (Prod M T) = (Srt s).
+Proof.
+  induction 1 ; simpl ; intros ;
+  auto with coc core arith datatypes ; try discriminate.
+
+  exists s1 ; exists s2.
+  exists U.
+  inversion H2.
+  rewrite <- H5 ; rewrite <- H6.
+  intuition.
+
+  simpl in IHtyp1 ; auto.
+  apply IHtyp1 ; auto.
+  apply (type_range_sub H2 H4).
+Qed.
+
+Lemma sort_of_abs_range : forall e M N Ts, e |- Abs M N : Ts ->
+  forall s, type_range Ts = Srt s ->
+  exists s1, exists s2, exists T, e |- M : (Srt s1) /\ M :: e |- N : T /\
+  M :: e |- T : Srt s2 /\ type_range T = (Srt s).
+Proof.
+  intros. 
+  apply sort_of_abs_range_aux with (Abs M N) Ts  ; auto ; auto.
+Qed.
 
 
-induction (prod_target_dec Ur (Ref 0)).
-induction a.
 
 
-cut (exists n, prod_target (subst v Ur) (n + x0)  
+Lemma sort_of_pair_range_aux : forall e t Ts, e |- t : Ts ->
+  forall T u v, t = Pair T u v ->
+  forall s, type_range Ts = Srt s ->
+  exists U, exists V, exists s1, exists s2,
+  T = Sum U V /\
+  e |- u : U /\ e |- U : Srt s1 /\ U :: e |- V : Srt s2 /\
+  e |- v : subst u V /\ e |- Sum U V : Srt s2 /\ 
+  type_range V = (Srt s).
+Proof.
+  induction 1 ; simpl ; intros ;
+  auto with coc core arith datatypes ; try discriminate.
 
-assert(prod_sort (subst v Ur) 
+  exists U ; exists V ; exists s1 ; exists s2.
+  inversion H3.
+  rewrite <- H7 ; rewrite <- H8.
+  intuition.
+  apply type_sum with s1 ; auto.
+  
+  apply IHtyp1 ; auto.
+  apply (type_range_sub H2 H4).
+Qed.
 
-Lemma unicity_sorting : forall G T s1, G |- T : Srt s1 ->
-  forall s2, G |- T : Srt s2 -> s1 = s2.
-Admitted.
+Lemma sort_of_pair_range : forall e T u v Ts, e |- Pair T u v : Ts ->
+  forall s, type_range Ts = Srt s ->
+  exists U, exists V, exists s1, exists s2,
+  T = Sum U V /\
+  e |- u : U /\ e |- U : Srt s1 /\ U :: e |- V : Srt s2 /\
+  e |- v : subst u V /\ e |- Sum U V : Srt s2 /\ 
+  type_range V = (Srt s).
+Proof.
+  intros. 
+  apply sort_of_pair_range_aux with (Pair T u v) Ts  ; auto ; auto.
+Qed.
+
+Lemma sort_of_pi1_range_aux : forall e t Ts, e |- t : Ts ->
+  forall u, t = Pi1 u ->
+  forall s, type_range Ts = Srt s ->
+  exists U, exists V, e |- u : Sum U V /\ type_range U = (Srt s).
+Proof.
+  induction 1 ; simpl ; intros ;
+  auto with coc core arith datatypes ; try discriminate.
+
+  exists U ; exists V.
+  inversion H0.
+  rewrite <- H3.
+  intuition.
+  
+  apply IHtyp1 ; auto.
+  apply (type_range_sub H2 H4).
+Qed.
+
+Lemma sort_of_pi1_range :  forall e t Ts, e |- Pi1 t : Ts ->
+  forall s, type_range Ts = Srt s ->
+  exists U, exists V, e |- t : Sum U V /\ type_range U = (Srt s).
+Proof.
+  intros. 
+  apply sort_of_pi1_range_aux with (Pi1 t) Ts  ; auto ; auto.
+Qed.
+
+Lemma sort_of_pi2_range_aux : forall e t Ts, e |- t : Ts ->
+  forall u, t = Pi2 u ->
+  forall s, type_range Ts = Srt s ->
+  exists U, exists V, e |- u : Sum U V /\ type_range (subst (Pi1 u) V) = (Srt s).
+Proof.
+  induction 1 ; simpl ; intros ;
+  auto with coc core arith datatypes ; try discriminate.
+
+  exists U ; exists V.
+  inversion H0.
+  rewrite <- H3.
+  intuition.
+  
+  apply IHtyp1 ; auto.
+  apply (type_range_sub H2 H4).
+Qed.
+
+Lemma sort_of_pi2_range :  forall e t Ts, e |- Pi2 t : Ts ->
+  forall s, type_range Ts = Srt s ->
+  exists U, exists V, e |- t : Sum U V /\ type_range (subst (Pi1 t) V) = (Srt s).
+Proof.
+  intros. 
+  apply sort_of_pi2_range_aux with (Pi2 t) Ts  ; auto ; auto.
+Qed.
+
+Lemma sort_of_letin_range_aux : forall e t Ts, e |- t : Ts ->
+  forall u v, t = Let_in u v ->
+  forall s, type_range Ts = Srt s ->
+  exists U, exists V, 
+  e |- u : U /\ U :: e |- v : V /\ 
+  type_range (subst u V) = (Srt s).
+Proof.
+  induction 1 ; simpl ; intros ;
+  auto with coc core arith datatypes ; try discriminate.
+
+  exists U ; exists M.
+  inversion H3.
+  rewrite <- H6 ; rewrite <- H7.
+  intuition.
+  
+  apply IHtyp1 ; auto.
+  apply (type_range_sub H2 H4).
+Qed.
+
+Lemma sort_of_letin_range :  forall e u v Ts, e |- Let_in u v : Ts ->
+  forall s, type_range Ts = Srt s ->
+  exists U, exists V,
+  e |- u : U /\ U :: e |- v : V /\
+  type_range (subst u V) = (Srt s).
+Proof.
+  intros. 
+  apply sort_of_letin_range_aux with (Let_in u v) Ts  ; auto ; auto.
+Qed.
+
+Lemma type_range_subst2 : forall t u n s, type_range t = Srt s -> 
+  type_range (subst_rec u t n) = Srt s.
+Proof.
+  induction t ; simpl ; intros ;
+  auto with coc core arith datatypes ; try discriminate.
+Qed.
+
+Lemma unique_range_sort : forall t e T T', e |- t : T -> e |- t : T' -> 
+forall s1 s2, 
+(type_range T = Srt s1 -> type_range T' = Srt s2 -> s1 = s2) /\
+(type_dom T = Srt s1 -> type_dom T' = Srt s2 -> s1 = s2).
+Proof.
+  induction t ; simpl ; split ; intros ;
+  auto with coc core arith datatypes ; try discriminate.
+
+  destruct (typ_sort _ _ _ H).
+  destruct (typ_sort _ _ _ H0).
+  rewrite H4 in H1.
+  rewrite H6 in H2.
+  simpl in H1, H2.
+  inversion H2 ; inversion H1.
+  auto.
+
+  destruct (typ_sort _ _ _ H).
+  destruct (typ_sort _ _ _ H0).
+  rewrite H4 in H1.
+  rewrite H6 in H2.
+  simpl in H1, H2.
+  inversion H2 ; inversion H1.
+  auto.
+
+  (* Var *)
+  exact (unique_var_range_sort H H1 H0 H2).
+  exact (unique_var_dom_sort H H1 H0 H2).
+    
+  (* Abs *)
+  induction (sort_of_abs_range H H1).
+  do 2 destruct H3 ; intuition.
+  induction (sort_of_abs_range H0 H2).
+  do 2 destruct H6 ; intuition.
+
+  destruct (IHt2 _ _ _ H3 H6 s1 s2) ; simpl ; auto.
+
+
+  destruct (IHt2 _ _ _ H3 H6 s1 s2) ; simpl ; auto.
+
+
+  (* App goes well *)
+  induction (sort_of_app_range H H1).
+  destruct H3 ; intuition.
+  induction (sort_of_app_range H0 H2).
+  destruct H6 ; intuition.
+
+  apply (IHt1 _ _ _ H3 H6) ; simpl ; auto.
+
+  pose (term_type_range_kinded H4 H8).
+  rewrite e0 in H3.
+  pose (type_no_kind_prod_type2 H3).
+  simpl in t.
+  intuition.
+
+  induction (sort_of_app_range H0 H2).
+  destruct H6 ; intuition.
+
+  apply (IHt1 _ _ _ H3 H6) ; simpl ; auto.
+
+  pose (term_type_range_kinded H4 H5).
+  rewrite e0 in H3.
+  pose (type_no_kind_prod_type2 H3).
+  simpl in t.
+  intuition.
+
+  pose (term_type_range_kinded H4 H5).
+  rewrite e0 in H3.
+  pose (type_no_kind_prod_type2 H3).
+  simpl in t.
+  intuition.
+
+  (* Pair *)
+  induction (sort_of_pair_range H H1).
+  do 3 destruct H3 ; intuition.
+  induction (sort_of_pair_range H0 H2).
+  do 3 destruct H9 ; intuition.
+
+  apply (IHt3 _ _ _ H7 H14) ; simpl ; auto.
+  unfold subst ; apply type_range_subst2 ; auto.
+  unfold subst ; apply type_range_subst2 ; auto.
+  
+  (* Prod *)
+  induction (generation_prod H).
+  induction (generation_prod H0).
+  rewrite H3 in H.
+  rewrite H4 in H0.
+  induction (generation_prod2 H).
+  induction (generation_prod2 H0).
+  apply (IHt2 _ _ _ H6 H8).
+  rewrite <- H3 ; auto.
+  rewrite <- H4 ; auto.
+
+  (* Sum *)
+  induction (generation_sum H).
+  induction (generation_sum H0).
+  rewrite H3 in H.
+  rewrite H4 in H0.
+  induction (generation_sum2 H).
+  induction (generation_sum2 H0).
+  apply (IHt2 _ _ _ H6 H8).
+  rewrite <- H3 ; auto.
+  rewrite <- H4 ; auto.
+  
+  pose (generation_subset H).
+  pose (generation_subset H0).
+  rewrite e0 in H1.
+  rewrite e1 in H2.
+  simpl in H1 ; simpl in H2.
+  rewrite H2 in H1.
+  inversion H1 ; auto.
+
+  (* Pi1 *)
+  induction (sort_of_pi1_range H H1).
+  destruct H3 ; intuition.
+  induction (sort_of_pi1_range H0 H2).
+  destruct H3 ; intuition.
+
+  apply (IHt _ _ _ H4 H6) ; simpl ; auto.
+
+  pose (term_type_range_kinded H4 H8).
+  rewrite e0 in H3.
+  pose (type_no_kind_prod_type2 H3).
+  simpl in t.
+  intuition.
+
+  induction (sort_of_app_range H0 H2).
+  destruct H6 ; intuition.
+
+  apply (IHt1 _ _ _ H3 H6) ; simpl ; auto.
+
+  pose (term_type_range_kinded H4 H5).
+  rewrite e0 in H3.
+  pose (type_no_kind_prod_type2 H3).
+  simpl in t.
+  intuition.
+
+  pose (term_type_range_kinded H4 H5).
+  rewrite e0 in H3.
+  pose (type_no_kind_prod_type2 H3).
+  simpl in t.
+  intuition.
+
+
+
+Admitted. 
+(* Focus 3.
+
+  split.
+  intros.
+  apply trans_conv_conv with A ; auto with coc core.
+
+  intros.
+  apply trans_conv_conv with B ; auto with coc core.
 *)
-(*
-Lemma coerce_trans : forall e T U, 
-  e |- T >> U -> 
-  forall s,
-  e |- T : Srt s ->
-  e |- U : Srt s ->
-  forall V, e |- V : Srt s ->
-  e |- U >> V ->
-  e |- T >> V.
+
+Theorem unique_sort : forall t e s s', 
+  e |- t : (Srt s) -> e |- t : (Srt s') -> s = s'.
 Proof.
-do 4 intro.
-induction H.
-intros ; assumption.
-intros.
-
-inversion_clear H6.
-apply coerce_prod with s ; auto with coc.
-
-pose (unicity_sorting HIHt H8).
-rewrite <- e in H7.
-pose (IHcoerce1 _ H H0 _ H7).
-
-apply coerce_prod with s ; auto with coc.
-
-*)
-
-
-
-
-
-
-
-
-
-
-
-
-
-
-
-
+  intros.
+  exact (unique_range_sort H H0 (refl_equal (Srt s)) (refl_equal (Srt s'))).
+Qed.
+  
+  
 
 
